refactor and add polymoprhic circuit_equiv

Gadgets.v
@@ -13,21 +13,18 @@ Module Gadgets.
 
   Include Stlc_Fp.
 
-  Definition X : atom := fresh nil.
-  Definition Y : atom := fresh (X :: nil).
-  
   (** Notation on Stlc_Ott *)
-  
   Coercion tm_var_f: expvar >-> exp.
   Coercion tm_constant: constant >-> exp.
   
   Declare Custom Entry stlc_ty.
   Declare Custom Entry stlc.
   Notation "'fp' n" := (const_field n) (in custom stlc at level 0).
+  Notation "'fb' b" := (const_bool b) (in custom stlc at level 0).
   Notation "'F0'" := (const_field fp_zero) (in custom stlc at level 0).
   Notation "'F1'" := (const_field fp_one) (in custom stlc at level 0).
-  Notation "'true'" := (const_true) (in custom stlc at level 0).
-  Notation "'false'" := (const_false) (in custom stlc at level 0).
+  Notation "'true'" := (const_bool true) (in custom stlc at level 0).
+  Notation "'false'" := (const_bool false) (in custom stlc at level 0).
   Notation "<{ e }>" := e (e custom stlc at level 99).
   Notation "<{{ e }}>" := e (e custom stlc_ty at level 99).
   Notation "( x )" := x (in custom stlc, x at level 99).
@@ -39,17 +36,18 @@ Module Gadgets.
   Notation "\_ : t , y" :=
     (tm_abs t y) (in custom stlc at level 90,
                      t custom stlc_ty at level 99,
-                     y custom stlc at level 99,
+                     y custom stlc at level 80,
                      left associativity).
   Notation "# n" := (tm_var_b n%nat) (in custom stlc at level 1).
   Notation "{ x }" := x (in custom stlc at level 1, x constr).
 
-  Notation "S -> T" := (ty_arrow S T) (in custom stlc_ty at level 0, right associativity).
+  Notation "S -> T" := (ty_arrow S T) (in custom stlc_ty at level 2, right associativity).
   Notation "Gamma '|-' t '::' T" := (typing Gamma t T) (in custom stlc_ty at level 40, t custom stlc, T custom stlc_ty at level 1).
                                                                        
   Notation "'Field'" := ty_field (in custom stlc_ty at level 0).
   Notation "'Bool'" := ty_bool (in custom stlc_ty at level 0).
-
+  Notation "a '*' b" := (ty_prod a b) (in custom stlc_ty at level 1, left associativity).
+  
   Notation "x + y" := (tm_binop x op_add y) (in custom stlc at level 2,
                                                 left associativity).
   Notation "x - y" := (tm_binop x op_sub y) (in custom stlc at level 2,
@@ -74,9 +72,16 @@ Module Gadgets.
                               z custom stlc at level 99,
                               left associativity).
 
-  Notation "'let _' '=' t1 'in' t2" :=
-    (tm_let t1 t2) (in custom stlc at level 0).
+  Notation "'let' t1 'in' t2" :=
+    (tm_let t1 t2) (in custom stlc at level 88,
+                       t1 custom stlc at level 99,
+                       t2 custom stlc at level 99,
+                   left associativity).
 
+  Notation "'{' a ',' b '}'" := (tm_pair a b) (in custom stlc at level 5, left associativity).
+  Notation "'fst' a" := (tm_proj_1 a) (in custom stlc at level 5).
+  Notation "'snd' a" := (tm_proj_2 a) (in custom stlc at level 5).
+  
   (** TR closure *)
   Inductive multi {X : Type} (R : relation X) : relation X :=
   | multi_refl : forall (x : X), multi R x x
@@ -87,175 +92,18 @@ Module Gadgets.
 
   Notation " t '-->*' t' " := (multi step t t') (at level 40).
 
-  (** Example 1: Division *)
-  Definition div :=
-    <{ \_: Field, (F1 / #0) }>.
-
-  Definition div_check :=
-    <{ \_: Field,
-           (\_: Field,
-                (#0 * #1) == F1)
-     }>.
-
-
   Definition circuit_equiv(c: exp) (c': exp): Prop :=
     forall (n: Fp), forall (w: Fp),
         (<{ c' (fp n) (fp w) }> -->* <{ true }> <->
-        <{ c (fp n) }> -->* <{ fp w }>).
-   
+        <{ c (fp n) }> -->* <{ fp w }>). 
   Notation "a '~~' b" := (circuit_equiv a b) (at level 50).
+
+  Definition circuit_equiv_poly(c: exp) (c': exp): Prop :=
+    forall n w T,
+      <{{ nil |- c n :: T }}> ->
+      <{{ nil |- c' n w :: Bool }}> ->
+      (<{ c' n w }> -->* <{ true }> <->
+       <{ c n }> -->* <{ w }>).
+  Notation "a ~= b" := (circuit_equiv_poly a b) (at level 99).
   
-  Ltac invert H := inversion H; subst; clear H.
-  Ltac invert_log_solved H g := 
-    solve [inversion H; fail; idtac "solved"] || invert H.
-
-  Lemma fp_mul_inv: forall n, n <> fp_zero -> pkmul (pkdiv fp_one n) n = fp_one.
-  Proof.
-    intros.
-    pose proof (pKfth p_prime) as FT.
-    invert FT.
-    rewrite Fdiv_def.
-    invert F_R.
-    rewrite <- Rmul_assoc.
-    rewrite Finv_l.
-    rewrite Rmul_1_l.
-    reflexivity.
-    assumption.
-  Qed.
-
-  Lemma fp_mul_div : forall n w, n <> fp_zero ->
-                               pkdiv (pkmul w n) n = w.
-  Proof.
-    intros.
-    pose proof (pKfth p_prime) as FT.
-    invert FT.
-    rewrite Fdiv_def.
-    invert F_R.
-    rewrite <- Rmul_assoc.
-    apply Finv_l in H.
-    replace (pkmul n (pkinv n)) with (pkmul (pkinv n) n) by (apply Rmul_comm).
-    rewrite H.
-    rewrite <- Rmul_comm.
-    rewrite Rmul_1_l.
-    reflexivity.
-  Qed.
-
-  Lemma neq_stlc_fp: forall n w, <{ fp n }> <> <{ fp w }> <-> n <> w.
-  Proof.
-    intro n.
-    destruct n as (n', n_mod).
-    induction n'; split; intros.
-    - intro. invert H0; contradiction.
-    - intro. invert H0; contradiction.
-    - intro. invert H0; contradiction.
-    - intro. invert H0; contradiction.
-    - intro. invert H0; contradiction.
-    - intro. invert H0; contradiction.
-  Qed.
-
-  Ltac solve_stlc :=
-    repeat match goal with
-           | [ H: step ?a ?b |- ?g ] => invert_log_solved H g
-           | [ H: ?a -->* ?b |- _ ] => inversion H; subst; clear H
-           | [ H: _ |- _ -->* _ ] => idtac "forward" ; econstructor; fail
-           | [ H: _ |- Is_true _ ] => idtac "is_true"; constructor
-           | [ H: ?x `notin` ?L |- lc_exp <{ \_: _, _ }> ] =>
-             idtac "intro binders"; apply (lc_tm_abs (AtomSetImpl.add ?x ?L));
-             intros; cbn ;econstructor                                                           
-           | [ H: _ |- lc_exp <{ \_ : _, _ }> ] =>
-             idtac "intro binders 2"; apply (lc_tm_abs empty);
-             intros; cbn; econstructor
-           | [ H: _ |- lc_exp _ ] => idtac "lc_exp"; constructor
-           end.
-
-     
-  Theorem div_gadget_equiv: div ~~ div_check.
-  Proof.
-    unfold circuit_equiv, div, div_check.
-    intros n w.
-    split; intro H; solve_stlc.
-    - destruct (eq_fp n fp_zero); econstructor.
-      (* n = 0 *)
-      eapply step_beta; solve_stlc.
-      cbn.
-      invert H9.          
-      cbn in H0.
-      rewrite Zmult_comm in H0.
-      pose proof (p_prime).
-      invert H.
-      rewrite Z.mod_0_l in H0.
-      rewrite Z.mod_1_l in H0.
-      invert H0.
-      assumption.
-      intro Hcontra.
-      rewrite Hcontra in H1.
-      invert H1.
-      (* n <> 0 *)
-      eapply step_beta; solve_stlc.
-      cbn.
-      econstructor.
-      apply step_div_const.
-      apply neq_stlc_fp.
-      assumption.
-      pose proof (fp_mul_div n w n0).      
-      rewrite -> H.
-      apply multi_refl.
-    - econstructor. 
-      eapply step_app_1. constructor. 
-      eapply step_beta.
-      econstructor.
-      apply (lc_tm_abs empty).
-      intros.
-      solve_stlc.
-      cbn.
-      solve_stlc.
-      econstructor.
-      cbn.
-      econstructor.
-      eapply step_beta; solve_stlc.
-      cbn.
-      econstructor.
-      apply step_eq_cog_1.
-      constructor.
-      eapply step_mul_const.
-      rewrite (fp_mul_inv).
-      econstructor.
-      eapply step_eq_refl.
-      apply multi_refl.
-      apply neq_stlc_fp.
-      assumption.
-  Qed.
- 
-  Fixpoint constant_to_boolnat(c: constant) : Fp :=
-    match c with
-    | const_true => fp_one
-    | const_false => fp_zero
-    | const_field (GZnZ.mkznz _ Z0 _) => fp_zero
-    | const_field (GZnZ.mkznz _ _ _) => fp_one
-    end.
-  
-  (** Example 2: Conditional *)
-  Definition ite(c: constant):=
-    <{ \_: Field,
-           (\_: Field,
-                if c then #0 else #1
-           )
-     }>.
-  
-  Definition ite_check(c: constant) :=
-    <{ \_: Field,
-           (\_: Field,
-                (\_: Field,
-                     (#2 == #0 + {constant_to_boolnat c} * (#1 - #0))
-                )
-           )
-     }>.
-
-  Theorem ite_equiv_2: forall c, ite c ~~ ite_check c.
-  Proof.
-    intros.
-    unfold circuit_equiv2, ite, ite_check.
-    intros; split; intro H; solve.
-  Qed.
-
-End Gadgets.     
+ End Gadgets.     
