DivGadget.v
@@ -1,0 +1,175 @@
+Require Import Metalib.Metatheory.
+From STLCZK Require Import Stlc.
+From STLCZK Require Import Gadgets.
+
+Require Import Coqprime.elliptic.ZEll.
+Require Import Coq.Numbers.BinNums.
+Require Import Coqprime.elliptic.GZnZ.
+Require Import Coq.ZArith.Znumtheory.
+Require Import Coq.ZArith.BinIntDef.
+Import Z.
+Require Import Coq.ZArith.BinInt.
+
+Module DivGadget.
+  Include Gadgets.
+
+  (** Example 1: Division *)
+  Definition div :=
+    <{ \_: Field, (F1 / #0) }>.
+
+  Definition div_check :=
+    <{ \_: Field,
+           (\_: Field,
+                (#0 * #1) == F1)
+     }>.
+  
+  Ltac invert H := inversion H; subst; clear H.
+  Ltac invert_log_solved H g := 
+    solve [inversion H; fail; idtac "solved"] || invert H.
+
+  Lemma fp_mul_inv: forall n, n <> fp_zero -> pkmul (pkdiv fp_one n) n = fp_one.
+  Proof.
+    intros.
+    pose proof (pKfth p_prime) as FT.
+    invert FT.
+    rewrite Fdiv_def.
+    invert F_R.
+    rewrite <- Rmul_assoc.
+    rewrite Finv_l.
+    rewrite Rmul_1_l.
+    reflexivity.
+    assumption.
+  Qed.
+
+  Lemma fp_mul_div : forall n w, n <> fp_zero ->
+                               pkdiv (pkmul w n) n = w.
+  Proof.
+    intros.
+    pose proof (pKfth p_prime) as FT.
+    invert FT.
+    rewrite Fdiv_def.
+    invert F_R.
+    rewrite <- Rmul_assoc.
+    apply Finv_l in H.
+    replace (pkmul n (pkinv n)) with (pkmul (pkinv n) n) by (apply Rmul_comm).
+    rewrite H.
+    rewrite <- Rmul_comm.
+    rewrite Rmul_1_l.
+    reflexivity.
+  Qed.
+
+  Lemma fp_mul_zero_l: forall w, (pkmul w fp_zero) = fp_zero.
+  Proof.
+    intros.
+    cbn.
+    apply GZnZ.zirr.
+    
+    rewrite Zmult_comm.
+    pose proof (p_prime).
+    invert H.
+    rewrite Z.mod_0_l.
+    cbn.
+    reflexivity.    
+    intro Hcontra.    
+    rewrite Hcontra in H0.
+    invert H0.
+  Qed.
+
+  Lemma neq_stlc_fp: forall n w, <{ fp n }> <> <{ fp w }> <-> n <> w.
+  Proof.
+    intro n.
+    destruct n as (n', n_mod).
+    induction n'; split; intros.
+    - intro. invert H0; contradiction.
+    - intro. invert H0; contradiction.
+    - intro. invert H0; contradiction.
+    - intro. invert H0; contradiction.
+    - intro. invert H0; contradiction.
+    - intro. invert H0; contradiction.
+  Qed.
+
+  Lemma mod_0_neq_1: 0 mod p <> 1 mod p.
+  Proof.
+    destruct (p_prime).
+    rewrite Z.mod_0_l.
+    rewrite Z.mod_1_l.
+    intro.
+    invert H1.
+    assumption.
+    intro.
+    rewrite H1 in H.
+    invert H.
+  Qed.
+
+  Ltac solve_stlc :=
+    repeat match goal with
+           | [ |- step (tm_eq ?a ?b) _ ] =>
+             apply step_eq_refl || apply step_eq_cog_1 || apply step_eq_cog_2
+           | [ |- step (tm_binop _ op_mul _) _ ] => apply step_mul_const
+           | [ |- step (tm_app ((tm_abs _ _))  _) _] => eapply step_beta
+           | [ H: step ?a ?b |- ?g ] => invert_log_solved H g
+           | [ H: ?a -->* ?b |- _ ] => inversion H; subst; clear H
+           | [ |- Is_true _ ] => idtac "is_true"; constructor
+           | [ H: ?x `notin` ?L |- lc_exp <{ \_: _, _ }> ] =>
+             idtac "intro binders"; apply (lc_tm_abs (AtomSetImpl.add ?x ?L)); intros
+           | [ |- lc_exp <{ \_ : _, _ }> ] =>
+             idtac "intro binders 2"; apply (lc_tm_abs empty); intros
+           | [ |- lc_exp _ ] => idtac "lc_exp"; constructor
+           | [ H: context[open_exp_wrt_exp _ _] |- _] => cbn in H
+           | [ |- context[open_exp_wrt_exp _ _] ] => cbn
+           | [ H: ?a |- ?a ] => exact H
+           | [ |- _ -->* _ ] => idtac "forward" ; econstructor; fail
+           end.
+
+  (** First equivalence proof, monomorphic to Field *)
+  Theorem div_gadget_equiv: div ~~ div_check.
+  Proof.
+    unfold circuit_equiv, div, div_check.
+    intros n w.
+    split; intro H; solve_stlc.
+    - destruct (eq_field n fp_zero); solve_stlc.
+      (* n = 0 *)
+      subst.
+      rewrite fp_mul_zero_l in H9.
+      invert H9.
+      apply mod_0_neq_1 in H0.
+      contradiction.
+      (* n <> 0 *)
+      econstructor; solve_stlc.
+      econstructor.
+      apply step_div_const.
+      generalize n0.
+      apply neq_stlc_fp.
+      rewrite -> (fp_mul_div n w n0).      
+      apply multi_refl.
+    - econstructor.
+      eapply step_app_1; solve_stlc.
+      cbn.
+      econstructor; try eapply step_beta; solve_stlc.
+      econstructor; solve_stlc.      
+      econstructor.
+      rewrite fp_mul_inv.
+      eapply step_eq_refl.
+      apply neq_stlc_fp.
+      assumption.
+      apply multi_refl.
+  Qed.
+
+  (** Second equivalence proof polymorphic *)
+  Theorem div_equiv_poly:
+      div ~= div_check.
+  Proof.
+    unfold circuit_equiv_poly, div, div_check.
+    intros n w T Tc Tc'.
+    invert Tc.
+    invert Tc'.
+    invert H2.
+    invert H3.
+    cbn in H1.
+    invert H5.
+    cbn in H2.
+    
+    split; intros; solve_stlc.
+  Admitted.
+
+End DivGadgets.     
