IteGadget.v
@@ -1,0 +1,57 @@
+Require Import Metalib.Metatheory.
+From STLCZK Require Import Stlc.
+From STLCZK Require Import Gadgets.
+
+Require Import Coqprime.elliptic.ZEll.
+Require Import Coq.Numbers.BinNums.
+Require Import Coqprime.elliptic.GZnZ.
+Require Import Coq.ZArith.Znumtheory.
+Require Import Coq.ZArith.BinIntDef.
+Import Z.
+Require Import Coq.ZArith.BinInt.
+
+Module IteGadget.
+  Include Gadgets.
+  
+  (** Example 2: Conditional *)
+  Definition ite :=
+    <{ \_: Bool,
+           \_: Field,
+               \_: Field,
+                    if #0 then #1 else #2
+     }>.
+  
+  Definition ite_check(c: constant) :=
+    <{ \_: Field,
+           \_: Bool,
+               \_: Field,
+                   \_: Field,
+                       #3 == #1 + #0 * (#2 - #1)
+                    
+     }>.
+
+  Definition ite_curried :=
+    <{ \_: Bool * Field * Field,
+           let fst (fst #0) in (* bool *)
+           let snd (fst #0) in (* field *)
+           let snd (#0) in (* field *)
+           if #1 then #2 else #3
+     }>.
+
+  Definition ite_check_curried :=
+    <{ \_: Bool * Field * Field * Field,
+           let fst (fst (fst #0)) in (* bool *)
+           let snd (fst (fst #0)) in (* field *)
+           let snd (fst #0) in       (* field *)
+           let snd #0 in             (* answer *)
+           #4 == #2 + #1 * (#3 - #2)
+     }>.
+  
+  Theorem ite_equiv: ite_curried ~~ ite_check_curried.
+  Proof.
+    intros.
+    unfold circuit_equiv, ite, ite_check.
+    intros; split; intro H; solve_stlc.
+  Qed.
+
+End Gadgets.     
